pipit/plugin-test/Plugin.Test.CoreLift.fst
@@ -4,6 +4,14 @@ open Pipit.Plugin.Interface
 module PPL = Pipit.Plugin.Lift
 module PPI = Pipit.Plugin.Interface
 
+module PXB = Pipit.Exp.Base
+module PSSB = Pipit.Sugar.Shallow.Base
+module PPS  = Pipit.Prim.Shallow
+module PPT  = Pipit.Prim.Table
+
+// Don't warn on local let-recs; they're only for testing
+#push-options "--warn_error -242"
+
 // Useful for testing:
 #push-options "--ext pipit:lift:debug"
 #push-options "--print_implicits --print_bound_var_types --print_full_names"
@@ -13,13 +21,221 @@ instance has_stream_int: Pipit.Sugar.Shallow.Base.has_stream int = {
   val_default = 0;
 }
 
-module PXB = Pipit.Exp.Base
-module PSSB = Pipit.Sugar.Shallow.Base
-module PPS  = Pipit.Prim.Shallow
-module PPT  = Pipit.Prim.Table
+// define fby primitive by manually lifting
+let fby (#a: eqtype) {| PSSB.has_stream a |} (dflt: a) (strm: a): a = dflt
+
+[@@core_lifted; core_of_source "Plugin.Test.CoreLift.fby" (ModeFun Static false (ModeFun Static false (ModeFun Static true (ModeFun Stream true Stream))))]
+let fby_core (ctx: PPT.context PPS.table) (#a: eqtype) {| PSSB.has_stream a |}
+  (dflt: a) (strm: PXB.exp PPS.table ctx (PSSB.shallow a)): PXB.exp PPS.table ctx (PSSB.shallow a) =
+  PXB.XFby dflt strm
+
+// let rec' (#a: eqtype) {| PSSB.has_stream a |} (f: a -> a): a = admit ()
+
+// rec can't currently be implemented here, because the contexts required for rec are a bit weird
+// [@@core_lifted; core_of_source "Plugin.Test.CoreLift.rec'" (ModeFun Static false (ModeFun Static false (ModeFun (ModeFun Stream true Stream) true Stream)))]
+// let rec_core (ctx: PPT.context PPS.table) (#a: eqtype) {| PSSB.has_stream a |}
+//   (f: PXB.exp PPS.table (PSSB.shallow a :: ctx) (PSSB.shallow a) -> PXB.exp PPS.table (PSSB.shallow a :: ctx) (PSSB.shallow a)): PXB.exp PPS.table ctx (PSSB.shallow a) =
+//   PXB.XMu (
+//     let x = PXB.XBase (PXB.XBVar 0) in
+//     f x)
+
 
 [@@source_mode (ModeFun Stream true Stream)]
-let eg_letincs_strm (x: int) =
+let eg_inc_left_strm (x: int) =
+  x + 1
+
+%splice[] (PPL.lift_tac1 "eg_inc_left_strm")
+
+[@@source_mode (ModeFun Stream true Stream)]
+let eg_inc_right_strm (x: int) =
+  1 + x
+
+%splice[] (PPL.lift_tac1 "eg_inc_right_strm")
+
+
+[@@source_mode (ModeFun Stream true Stream)]
+let eg_additions_strm (x: int) =
   (x + x) + x
 
-%splice[eg_letincs_strm_core] (PPL.lift_tac "eg_letincs_strm" "eg_letincs_strm_core" (ModeFun Stream true Stream))
+%splice[] (PPL.lift_tac1 "eg_additions_strm")
+
+[@@source_mode (ModeFun Stream true Stream)]
+let eg_additions_strm_ret_ann (x: int): int =
+  (x + x) + x
+
+%splice[] (PPL.lift_tac1 "eg_additions_strm_ret_ann")
+
+
+
+[@@source_mode (ModeFun Stream true Stream)]
+let eg_fby (x: int) =
+  0 `fby` x
+
+%splice[] (PPL.lift_tac1 "eg_fby")
+
+
+[@@source_mode (ModeFun Stream true Stream)]
+let eg_fby_inc (x: int) =
+  0 `fby` x + 1
+
+%splice[] (PPL.lift_tac1 "eg_fby_inc")
+
+[@@source_mode (ModeFun Stream true Stream)]
+let eg_letrecfun (x: int): int =
+  let rec count x = if x > 0 then count (x - 1) else 0 in
+  count 0
+
+%splice[] (PPL.lift_tac1 "eg_letrecfun")
+
+[@@source_mode (ModeFun Stream true Stream)]
+let eg_let_strm (x: int): int =
+  let strm = x + 1 in
+  strm + x
+
+%splice[] (PPL.lift_tac1 "eg_let_strm")
+
+[@@source_mode (ModeFun Stream true Stream)]
+let eg_let_strm_ann (x: int): int =
+  [@@source_mode Stream]
+  let strm = 1 in
+  strm + x
+
+%splice[] (PPL.lift_tac1 "eg_let_strm_ann")
+
+[@@source_mode (ModeFun Stream true Stream)]
+let eg_rec_strm (x: int) =
+  let count = rec' (fun count -> 0 `fby` count + 1) in
+  count
+
+%splice[] (PPL.lift_tac1 "eg_rec_strm")
+
+// [@@Tac.preprocess_with preprocess; source]
+// let eg_mixed_ann (x: stream int): stream int =
+//   let rec count1 = 0 `fby` count1 + 1 in
+//   let rec count2: stream int = 0 `fby` count2 + 1 in
+//   let strm1: stream int = 0 in
+//   let strm2 = 0 <: stream int in
+//   let strm3 = count1 + strm1 in
+//   let static1: int = 0 in
+//   let static2 = 0 in
+//   count1 + count2 + strm1 + strm2 + strm3 + static1 + static2
+
+// %splice[] (autolift_binds [`%eg_mixed_ann])
+
+// let eg_pairs (x: stream int) (y: stream bool): stream int =
+//   0 `fby` fst (Mktuple2 x y)
+
+// %splice[] (autolift_binds [`%eg_pairs])
+
+
+// type ctor = | Ctor: x: int -> y: int -> ctor
+// instance has_stream_ctor: Shallow.has_stream ctor = {
+//   ty_id       = [`%ctor];
+//   val_default = Ctor Shallow.val_default Shallow.val_default;
+// }
+
+// [@@Tac.preprocess_with preprocess]
+// let eg_ctor (add: stream int): stream ctor =
+//   let rec rcd =
+//     let x = 0 `fby` Ctor?.x rcd + add in
+//     let y = 0 `fby` Ctor?.y rcd - add in
+//     Ctor x y
+//   in
+//   rcd
+
+// %splice[] (autolift_binds [`%eg_ctor])
+
+// [@@Tac.preprocess_with preprocess]
+// let eg_pairsrec (add: stream int): stream (int & int) =
+//   // recursive streams sometimes need annotations
+//   let rec xy: stream (int & int) =
+//     let x = 0 `fby` fst xy + add in
+//     let y = 0 `fby` snd xy - add in
+//     (x, y)
+//   in
+//   xy
+
+// %splice[] (autolift_binds [`%eg_pairsrec])
+
+// type record = { x: int; y: int; }
+
+// instance has_stream_record: Shallow.has_stream record = {
+//   ty_id       = [`%record];
+//   val_default = { x = 0; y = 0; };
+// }
+
+
+// // XXX:TODO: preprocess breaks on records?
+// [@@Tac.preprocess_with preprocess; source]
+// let eg_record (add: stream int): stream int =
+//   let x = 0 `fby` add in
+//   let y = 1 `fby` add in
+//   let xy = { x; y } in
+//   xy.x
+
+
+// %splice[] (autolift_binds [`%eg_record])
+
+// let eg_streaming_if (x: stream int): stream int =
+//   if x >= 0 then x else -x
+
+// %splice[] (autolift_binds [`%eg_streaming_if])
+
+// let eg_streaming_match_lets (x: stream int): stream int =
+//   let cond = x >= 0 in
+//   let abs =
+//     match cond with
+//       | true -> x
+//       | false -> -x
+//   in abs
+
+// %splice[] (autolift_binds [`%eg_streaming_match_lets])
+
+// let eg_static_match (consts: list int) (x: stream int): stream int =
+//   match consts with
+//   | [] -> 0
+//   | (c: int) :: _ -> c + x
+
+// %splice[] (autolift_binds [`%eg_static_match])
+
+// let silly_id (x: int): y: int { x == y } = x
+
+// (*** Examples / test cases ***)
+// [@@source]
+// let eg_refinement0 (x: stream int): stream int =
+//   silly_id x
+
+// %splice[] (autolift_binds [`%eg_refinement0])
+
+(*** Not supported examples ***)
+
+
+// mutual recursion not supported:
+
+// [@@Tac.preprocess_with tac_lift]
+// let eg_letrec_mut (x: int): int =
+//   let rec a = x + b
+//       and b = x - a
+//   in a
+
+// streaming matches cannot bind variables:
+
+// [@@Tac.preprocess_with tac_lift]
+// let eg_streaming_match_bind (x: stream (option int)): stream int =
+//   match x with
+//   | Some e -> e
+//   | None -> 0
+
+// [@@Tac.preprocess_with tac_lift]
+// let eg_streaming_letmatch (xy: stream (int & int)): stream int =
+//   let (x, y) = xy in
+//   x + y
+
+// Lemma instantiation not supported; use a pattern instead
+// let lemma_nat_something (x: int) (y: int): Lemma (ensures x > y) = admit ()
+
+// let eg_instantiate_lemma (x y: stream int): stream int =
+//   lemma_nat_something x y;
+//   x + y
+
+// %splice[] (autolift_binds [`%eg_instantiate_lemma])
